New style for finding transformations. See msg.
Previously the part of the code that found the transformation was part
of the code that needed to be verified, with proofs written directly
upon it. Now instead, we allow for an unverified function to find a
transformation for us, and then we simply prove the part that performs
a suggested transformation. In particular, this code that finds a
transformation for us is now [irreducible] and nothing is known about
it, other than the fact that it returns an object that contains
[possibly transformation_hints]. This means that no proof relies upon
this function, but instead, we have the main proof rely upon
[perform_transformation_with_hint] and
[perform_transformations_with_hint].

There are numerous advantages to this approach:
(1) Proofs no longer need to be updated as we try different heuristics
    for performing the unblocking.
(2) Once we have a "default" [find_transformation_hints], we are still
    not limited by it, since someone could easily come along and write
    their own [find_transformation_hints] (or even produce their own
    [transformation_hints] object manually) and pass it into the
    framework to perform the transformation.

The disadvantages to this approach are fairly minimal. In particular,
we can no longer find and perform the transformation at the same time,
but instead must do it separately. This should not be an issue, since
earlier too, we were (effectively) doing it in two steps.

vale/code/lib/transformers/Vale.Transformers.InstructionReorder.fst
@@ -1577,79 +1577,83 @@ let rec lemma_num_blocks_in_codes_append (c1 c2:codes) :
   | [] -> ()
   | x :: xs -> lemma_num_blocks_in_codes_append xs c2
 
-let rec unblock_for (c:code) (cs : codes) :
-  Pure (possibly codes)
-    (requires True)
-    (ensures (fun r ->
-         Ok? r ==> (
-           (Ok? (find_code c cs) ==> num_blocks_in_codes cs = num_blocks_in_codes (Ok?.v r)) /\
-           (Err? (find_code c cs) ==> num_blocks_in_codes cs > num_blocks_in_codes (Ok?.v r))))) =
-  match find_code c cs with
-  | Ok _ -> Ok cs
-  | Err _ -> (
-      match cs with
-      | [] -> Err "Cannot unblock further"
-      | Block l :: xs -> (
-          match unblock_for c l with
-          | Ok l' -> Ok (l' `L.append` xs)
-          | Err r -> (
-              xs' <-- unblock_for c xs;
-              return (Block l :: xs')
-            )
+type transformation_hint =
+  | MoveUpFrom : p:nat -> transformation_hint
+  | DiveInAt : p:nat -> q:transformation_hint -> transformation_hint
+
+type transformation_hints = list transformation_hint
+
+let rec string_of_transformation_hint (t:transformation_hint) : string =
+  match t with
+  | MoveUpFrom p -> "(MoveUpFrom " ^ string_of_int p ^ ")"
+  | DiveInAt p q -> "(DiveInAt " ^ string_of_int p ^ " " ^ string_of_transformation_hint q ^ ")"
+
+irreducible
+(* Our proofs do not depend on how the hints are found. As long as
+   some hints are provided, we validate the hints to perform the
+   transformation and use it. Thus, we make this function
+   [irreducible] to explicitly prevent any of the proofs from
+   reasoning about it. *)
+let rec find_transfomation_hints (c1 c2:codes) : possibly transformation_hints =
+  Err "temp. no transformation found. TODO FIXME"
+
+(* XXX: Copied from List.Tot.Base because of an extraction issue.
+   See https://github.com/FStarLang/FStar/pull/1822. *)
+val split3: #a:Type -> l:list a -> i:nat{i < L.length l} -> Tot (list a * a * list a)
+let split3 #a l i =
+  let a, as = L.splitAt i l in
+  L.lemma_splitAt_snd_length i l;
+  let b :: c = as in
+  a, b, c
+
+let rec perform_reordering_with_hint (t:transformation_hint) (c:codes) : possibly codes =
+  match c with
+  | [] -> Err "trying to transform empty code"
+  | x :: xs -> (
+      match t with
+      | MoveUpFrom i -> (
+          if i < L.length c then (
+            c' <-- bubble_to_top c i;
+            return (L.index c i :: c')
+          ) else (
+            Err ("invalid hint : " ^ string_of_transformation_hint t)
+          )
         )
-      | x :: xs ->
-        xs' <-- unblock_for c xs;
-        return (x :: xs')
+      | DiveInAt i t' ->
+        if i < L.length c then (
+          FStar.List.Pure.lemma_split3_length c i;
+          let left, mid, right = split3 c i in
+          match mid with
+          | Block l ->
+            l' <-- perform_reordering_with_hint t' l; (
+              match l' with
+              | [] -> Err "impossible"
+              | y :: ys ->
+                L.append_length left [y];
+                left' <-- bubble_to_top (left `L.append` [y]) i;
+                return (y :: (left' `L.append` (Block ys :: right)))
+            )
+          | _ ->
+            Err ("trying to dive into a non-block : " ^ string_of_transformation_hint t ^ " " ^ fst (print_code (Block c) 0 gcc))
+        ) else (
+          Err ("invalid hint : " ^ string_of_transformation_hint t)
+        )
     )
 
-let rec reordering_allowed (c1 c2 : codes) :
-  Tot pbool
-    (decreases %[c2; num_blocks_in_codes c1]) =
-  match c1, c2 with
-  | [], [] -> ttrue
-  | [], _ | _, [] -> ffalse "disagreeing lengths of codes"
-  | _, h2 :: t2 ->
-    match find_code h2 c1 with
-    | Ok i -> (
-        t1 <-- bubble_to_top c1 i;
-        reordering_allowed t1 t2
-      )
-    | Err reason -> (
-        let h1 :: t1 = c1 in
-        match h1, h2 with
-        | Block l1, Block l2 ->
-          reordering_allowed l1 l2 &&. reordering_allowed t1 t2
-        | _ -> (
-            match unblock_for h2 c1 with
-            | Ok c1' ->
-              reordering_allowed c1' c2 (* TODO: Handle IfElse and While specially too? *)
-            | Err _ -> Err reason
-          )
-      )
-
-(** Transform [c1] into the ordering specified by [c2] *)
-let rec perform_reordering (c1 c2 : codes) :
-  Pure (codes)
-    (requires !!(reordering_allowed c1 c2))
-    (ensures (fun c_gen -> eq_codes c_gen c2))
-    (decreases %[c2; num_blocks_in_codes c1]) =
-  match c1, c2 with
-  | [], [] -> []
-  | _, h2 :: t2 ->
-    match find_code h2 c1 with
-    | Ok i -> (
-        let Ok t1 = bubble_to_top c1 i in
-        L.index c1 i :: perform_reordering t1 t2
-      )
-    | Err _ -> (
-        let h1 :: t1 = c1 in
-        match h1, h2 with
-        | Block l1, Block l2 ->
-          assert (eq_code (Block (perform_reordering l1 l2)) (Block l2)); (* OBSERVE *)
-          Block (perform_reordering l1 l2) :: perform_reordering t1 t2
-        | _ ->
-          perform_reordering (Ok?.v (unblock_for h2 c1)) c2
-      )
+let rec perform_reordering_with_hints (ts:transformation_hints) (c:codes) : possibly codes =
+  match ts with
+  | [] -> (
+      match c with
+      | [] -> return []
+      | _ -> Err ("no more transformation hints for " ^ fst (print_code (Block c) 0 gcc))
+    )
+  | t :: ts' ->
+    c' <-- perform_reordering_with_hint t c;
+    match c' with
+    | [] -> Err "impossible"
+    | x :: xs ->
+      xs' <-- perform_reordering_with_hints ts' xs;
+      return (x :: xs')
 
 /// If there are two sequences of instructions that can be transformed
 /// amongst each other, then they behave identically as per the
@@ -1704,93 +1708,110 @@ let rec lemma_machine_eval_codes_block_to_append (c1 c2 : codes) (fuel:nat) (s:m
       lemma_machine_eval_codes_block_to_append xs c2 fuel s1
 #pop-options
 
-let rec lemma_unblock_for (c:code) (cs:codes) (fuel:nat) (s:machine_state) :
+let rec lemma_append_single (xs:list 'a) (y:'a) (i:nat) :
   Lemma
-    (requires (Ok? (unblock_for c cs)))
+    (requires (i == L.length xs))
     (ensures (
-        let Ok cs' = unblock_for c cs in
-        machine_eval_codes cs fuel s == machine_eval_codes cs' fuel s)) =
-  match find_code c cs with
-  | Ok _ -> ()
-  | Err _ -> (
-      match cs with
-      | Block l :: xs -> (
-          match unblock_for c l with
-          | Ok l' -> (
-              lemma_unblock_for c l fuel s;
-              assert (machine_eval_code (Block l) fuel s == machine_eval_code (Block l') fuel s);
-              assert (machine_eval_codes (Block l :: xs) fuel s == machine_eval_codes (Block l' :: xs) fuel s);
-              assert (machine_eval_codes cs fuel s == machine_eval_codes (Block l' :: xs) fuel s);
-              lemma_machine_eval_codes_block_to_append l' xs fuel s;
-              assert (machine_eval_codes cs fuel s == machine_eval_codes (l' `L.append` xs) fuel s)
-            )
-          | Err _ -> (
-              match machine_eval_code (Block l) fuel s with
-              | None -> ()
-              | Some s1 ->
-                lemma_unblock_for c xs fuel s1
-            )
-        )
-      | x :: xs -> (
-          match machine_eval_code x fuel s with
-          | None -> ()
-          | Some s1 ->
-            lemma_unblock_for c xs fuel s1
-        )
-    )
+        L.length (xs `L.append` [y]) = L.length xs + 1 /\
+        L.index (xs `L.append` [y]) i == y)) =
+  match xs with
+  | [] -> ()
+  | x :: xs -> lemma_append_single xs y (i - 1)
 
-let rec lemma_reordering (c1 c2 : codes) (fuel:nat) (s1 : machine_state) :
+#push-options "--z3rlimit 20 --initial_fuel 3 --max_fuel 3 --initial_ifuel 1 --max_ifuel 1"
+let rec lemma_perform_reordering_with_hint (t:transformation_hint) (cs:codes) (fuel:nat) (s:machine_state) :
   Lemma
     (requires (
-        !!(reordering_allowed c1 c2) /\
-        (Some? (machine_eval_codes c1 fuel s1)) /\
-        (Some?.v (machine_eval_codes c1 fuel s1)).ms_ok))
+        (Ok? (perform_reordering_with_hint t cs)) /\
+        (Some? (machine_eval_codes cs fuel s)) /\
+        (Some?.v (machine_eval_codes cs fuel s)).ms_ok))
     (ensures (
-        (Some? (machine_eval_codes (perform_reordering c1 c2) fuel s1)) /\
-        (let Some s1', Some s2' =
-           machine_eval_codes c1 fuel s1,
-           machine_eval_codes (perform_reordering c1 c2) fuel s1 in
-         equiv_states_or_both_not_ok s1' s2')))
-    (decreases %[c2; num_blocks_in_codes c1]) =
-  match c2 with
+        let Ok cs' = perform_reordering_with_hint t cs in
+        equiv_ostates
+          (machine_eval_codes cs fuel s)
+          (machine_eval_codes cs' fuel s))) =
+  let c = cs in
+  let Ok cs' = perform_reordering_with_hint t cs in
+  let Some s' = machine_eval_codes cs fuel s in
+  let x :: xs = cs in
+  match t with
+  | MoveUpFrom i -> (
+      let Ok c' = bubble_to_top c i in
+      lemma_bubble_to_top c i fuel s s'
+    )
+  | DiveInAt i t' -> (
+      FStar.List.Pure.lemma_split3_append c i;
+      FStar.List.Pure.lemma_split3_length c i;
+      let left, mid, right = L.split3 c i in
+      let Block l = mid in
+      let Ok (y :: ys) = perform_reordering_with_hint t' l in
+      L.append_length left [y];
+      let Ok left' = bubble_to_top (left `L.append` [y]) i in
+      //
+      assert (cs' == y :: (left' `L.append` (Block ys :: right)));
+      assert (left `L.append` (mid :: right) == c);
+      L.append_l_cons mid right left;
+      assert ((left `L.append` [mid]) `L.append` right == c);
+      lemma_machine_eval_codes_block_to_append (left `L.append` [mid]) right fuel s;
+      let Some s_1 = machine_eval_code (Block (left `L.append` [mid])) fuel s in
+      assert (Some s_1 == machine_eval_codes (left `L.append` [mid]) fuel s);
+      lemma_machine_eval_codes_block_to_append left [mid] fuel s;
+      let Some s_2 = machine_eval_code (Block left) fuel s in
+      assert (Some s_2 == machine_eval_codes left fuel s);
+      //
+      assert (Some s_1 == machine_eval_codes [mid] fuel s_2);
+      assert (Some s_1 == machine_eval_code (Block l) fuel s_2);
+      assert (Some s_1 == machine_eval_codes l fuel s_2);
+      assert (Some s' == machine_eval_codes right fuel s_1);
+      if s_1.ms_ok then () else lemma_not_ok_propagate_codes right fuel s_1;
+      lemma_perform_reordering_with_hint t' l fuel s_2;
+      //
+      let Some s_11 = machine_eval_codes (y :: ys) fuel s_2 in
+      let Some s_12 = machine_eval_code y fuel s_2 in
+      if s_12.ms_ok then () else lemma_not_ok_propagate_codes ys fuel s_12;
+      assert (Some s_2 == machine_eval_codes left fuel s);
+      assert (Some s_2 == machine_eval_code (Block left) fuel s);
+      assert (Some s_12 == machine_eval_codes (Block left :: [y]) fuel s);
+      lemma_machine_eval_codes_block_to_append left [y] fuel s;
+      assert (Some s_12 == machine_eval_codes (left `L.append` [y]) fuel s);
+      lemma_bubble_to_top (left `L.append` [y]) i fuel s s_12;
+      //
+      lemma_append_single left y i;
+      assert (L.index (left `L.append` [y]) i == y);
+      //
+      let Some s_3 = machine_eval_codes (y :: left') fuel s in
+      assert (equiv_states s_3 s_12);
+      lemma_eval_codes_equiv_states right fuel s_1 s_11;
+      let Some s_0 = machine_eval_codes right fuel s_11 in
+      lemma_eval_codes_equiv_states (Block ys :: right) fuel s_12 s_3;
+      let Some s_00 = machine_eval_codes (Block ys :: right) fuel s_3 in
+      //
+      assert (equiv_states s_00 s');
+      assert (Some s_3 == machine_eval_code (Block (y :: left')) fuel s);
+      assert (Some s_00 == machine_eval_codes (Block ys :: right) fuel s_3);
+      lemma_machine_eval_codes_block_to_append (y :: left') (Block ys :: right) fuel s
+    )
+#pop-options
+
+let rec lemma_perform_reordering_with_hints (ts:transformation_hints) (cs:codes) (fuel:nat) (s:machine_state) :
+  Lemma
+    (requires (
+        (Ok? (perform_reordering_with_hints ts cs)) /\
+        (Some? (machine_eval_codes cs fuel s)) /\
+        (Some?.v (machine_eval_codes cs fuel s)).ms_ok))
+    (ensures (
+        let Ok cs' = perform_reordering_with_hints ts cs in
+        equiv_ostates
+          (machine_eval_codes cs fuel s)
+          (machine_eval_codes cs' fuel s))) =
+  let c = cs in
+  let Ok cs' = perform_reordering_with_hints ts cs in
+  let Some s' = machine_eval_codes cs fuel s in
+  match ts with
   | [] -> ()
-  | h2 :: t2 ->
-    let c_gen = perform_reordering c1 c2 in
-    match find_code h2 c1 with
-    | Ok i -> (
-        let Ok t1 = bubble_to_top c1 i in
-        let h' = L.index c1 i in
-        let t' = perform_reordering t1 t2 in
-        lemma_bubble_to_top c1 i fuel s1 (Some?.v (machine_eval_codes c1 fuel s1));
-        let Some sa1' = machine_eval_code h' fuel s1 in
-        let Some sa2' = machine_eval_codes t1 fuel sa1' in
-        lemma_reordering t1 t2 fuel sa1'
-      )
-    | Err _ -> (
-        let h1 :: t1 = c1 in
-        match h1, h2 with
-        | Block l1, Block l2 ->
-          assert (machine_eval_code (Block l1) fuel s1 == machine_eval_codes l1 fuel s1);
-          assert (machine_eval_code (Block l2) fuel s1 == machine_eval_codes l2 fuel s1);
-          assert (Some? (machine_eval_code (Block l1) fuel s1));
-          assert (Some? (machine_eval_codes l1 fuel s1));
-          let Some s1' = machine_eval_codes l1 fuel s1 in
-          if s1'.ms_ok then () else (
-            lemma_not_ok_propagate_codes t1 fuel s1'
-          );
-          lemma_reordering l1 l2 fuel s1;
-          let Some s1'' = machine_eval_codes (perform_reordering l1 l2) fuel s1 in
-          assert (Some s1'' == machine_eval_code (Block (perform_reordering l1 l2)) fuel s1);
-          lemma_reordering t1 t2 fuel s1';
-          lemma_eval_codes_equiv_states (perform_reordering t1 t2) fuel s1' s1'';
-          let Some s2 = machine_eval_codes c1 fuel s1 in
-          let Some s2' = machine_eval_codes t1 fuel s1' in
-          let Some s2'' = machine_eval_codes (perform_reordering t1 t2) fuel s1'' in
-          assert (equiv_states s2 s2');
-          assert (equiv_states s2' s2'');
-          assert (machine_eval_codes (perform_reordering c1 c2) fuel s1 == machine_eval_codes (perform_reordering t1 t2) fuel s1'');
-          assert (Some s2'' == machine_eval_codes (perform_reordering c1 c2) fuel s1)
-        | _ ->
-          lemma_unblock_for h2 c1 fuel s1;
-          lemma_reordering (Ok?.v (unblock_for h2 c1)) c2 fuel s1
-      )
+  | t :: ts' ->
+    let Ok (x :: xs) = perform_reordering_with_hint t c in
+    lemma_perform_reordering_with_hint t c fuel s;
+    let Ok xs' = perform_reordering_with_hints ts' xs in
+    let Some s1 = machine_eval_code x fuel s in
+    lemma_perform_reordering_with_hints ts' xs fuel s1
